theories/binary_search_verif.v
@@ -1,19 +1,23 @@
-Require Import VST.floyd.proofauto. (* Import the Verifiable C system *)
-Require Import VST.floyd.sublist.
-Require Import VSTArrayProgs.binary_search. (* Import the AST of this C program *)
-Require Import Lia.
+From VST Require Import floyd.proofauto floyd.sublist.
+From VSTArrayProgs Require Import binary_search.
 
 Ltac do_compute_expr_warning::=idtac.
 
-(* The next line is "boilerplate", always required after importing an AST. *)
 Instance CompSpecs : compspecs. make_compspecs prog. Defined.
 Definition Vprog : varspecs.  mk_varspecs prog. Defined.
 
 Fixpoint sorted (l : list Z) : Prop :=
+  match l with
+  | [] => True
+  | x::rest =>
+    match rest with [] => True | y::_ =>  x <= y /\ sorted rest end
+  end.
+
+Fixpoint sorted' (l : list Z) : Prop :=
 match l with
 | [] => True
 | _ :: [] => True
-| x :: y :: l' => x <= y /\ sorted l'
+| x :: y :: l' => x <= y /\ sorted' l'
 end.
 
 Definition insertion_point (ip : Z) (key : Z) (l : list Z) :=
@@ -62,6 +66,141 @@ Proof.
   apply sublist_nil_gen.
 Qed.
 
+Lemma Znth_In : forall A (d: Inhabitant A) i (l : list A) x (Hrange : 0 <= i < Zlength l)
+ (Hnth : Znth i l = x), In x l.
+Proof.
+  unfold Znth; intros.
+  destruct (zlt i 0); [lia|].
+  subst; apply nth_In.
+  rewrite Zlength_correct in Hrange; auto.
+  rep_lia.
+Qed.
+
+Lemma In_Znth : forall A (d: Inhabitant A) (l : list A) x,
+    In x l ->
+    exists i, 0 <= i < Zlength l /\ Znth i l = x.
+Proof.
+  unfold Znth; intros.
+  apply In_nth with (d := d) in H; destruct H as (n & ? & ?).
+  exists (Z.of_nat n); split.
+  - rewrite Zlength_correct; lia.
+  - destruct (zlt (Z.of_nat n) 0); [lia|].
+    rewrite Nat2Z.id; auto.
+Qed.
+
+Lemma sublist_of_nil : forall A i j, sublist i j (nil : list A) = [].
+Proof.
+  intros; unfold sublist.
+  rewrite firstn_nil, skipn_nil; auto.
+Qed.
+
+Fixpoint sorted2 l :=
+  match l with
+  | [] => True
+  | x :: rest => Forall (fun y => x <= y) rest /\ sorted2 rest
+  end.
+
+Lemma sorted_equiv : forall l, sorted l <-> sorted2 l.
+Proof.
+  induction l; simpl.
+  - reflexivity.
+  - destruct l.
+    + simpl; split; auto.
+    + rewrite IHl; simpl; split; intros (? & Hall & ?); split3; auto.
+       * constructor; auto.
+          rewrite Forall_forall in *; intros ? Hin.
+          specialize (Hall _ Hin); lia.
+       * inversion H. auto.
+Qed.
+
+Lemma sorted_mono : forall l i j (Hsort : sorted l) (Hi : 0 <= i <= j)
+                           (Hj : j < Zlength l),
+    Znth i l <= Znth j l.
+Proof.
+induction l; intros.
+* rewrite !Znth_nil. lia.
+* 
+ rewrite sorted_equiv in Hsort. destruct Hsort as [H9 Hsort].
+ rewrite <- sorted_equiv in Hsort. rewrite Forall_forall in H9.
+ rewrite Zlength_cons in Hj.
+ destruct (zeq i 0).
+ +
+   subst i; rewrite Znth_0_cons. 
+   destruct (zeq j 0).
+   - subst j. rewrite Znth_0_cons. lia.
+   - rewrite Znth_pos_cons by lia.
+      apply H9.
+      eapply Znth_In; [ | reflexivity]; lia.
+ +
+    rewrite !Znth_pos_cons by lia.
+    apply IHl; auto; lia.
+Qed.
+
+Lemma In_sorted_range : forall lo hi x l (Hsort : sorted l) (Hlo : 0 <= lo <= hi)
+                              (Hhi : hi <= Zlength l)
+                              (Hin : In x (sublist lo hi l)),
+    Znth lo l <= x <= Znth (hi - 1) l.
+Proof.
+  intros.
+  generalize (In_Znth _ _ _ _ Hin); intros (i & Hrange & Hi).
+  rewrite Zlength_sublist in Hrange by auto.
+  rewrite Znth_sublist in Hi by lia.
+  subst; split; apply sorted_mono; auto; lia.
+Qed.
+
+Lemma In_sorted_gt : forall x i n l lo hi (Hsort : sorted l) (Hlo : lo >= 0)
+                            (Hhi : hi <= Zlength l)
+                            (Hin : In x (sublist lo hi l))
+                            (Hi : lo <= i < hi) (Hn : Znth i l = n)
+                            (Hgt : n < x),
+    In x (sublist (i + 1) hi l).
+Proof.
+  intros.
+  rewrite sublist_split with (mid := i + 1) in Hin; try lia.
+  rewrite in_app in Hin; destruct Hin; auto.
+  generalize (In_sorted_range lo (i + 1) x _ Hsort); intro X.
+  repeat (lapply X; [clear X; intro X | lia]).
+  replace (i + 1 - 1) with i in X by lia.
+  specialize (X H); subst; lia.
+Qed.
+
+Lemma In_sorted_lt : forall x i n l lo hi (Hsort : sorted l) (Hlo : lo >= 0)
+                            (Hhi : hi <= Zlength l)
+                            (Hin : In x (sublist lo hi l))
+                            (Hi : lo <= i < hi) (Hn : Znth i l = n)
+                            (Hgt : x < n),
+    In x (sublist lo i l).
+Proof.
+  intros.
+  rewrite sublist_split with (mid := i) in Hin; try lia.
+  rewrite in_app in Hin; destruct Hin; auto.
+  generalize (In_sorted_range i hi x _ Hsort); intro X.
+  repeat (lapply X; [clear X; intro X | lia]).
+  specialize (X H); subst; lia.
+Qed.
+
+Lemma Znth_In_sublist : forall A (d: Inhabitant A) i (l : list A) lo hi
+  (Hlo : 0 <= lo <= i) (Hhi : i < hi <= Zlength l),
+  In (Znth i l) (sublist lo hi l).
+Proof.
+  intros.
+  apply Znth_In with (i := i - lo)(d := d).
+  - rewrite Zlength_sublist; lia.
+  - rewrite <- (Z.sub_simpl_r i lo) at 2.
+    apply Znth_sublist; lia.
+Qed.
+
+Lemma sublist_In_sublist : forall A (l : list A) x lo hi lo' hi' (Hlo : 0 <= lo <= lo')
+  (Hhi : hi' <= hi), In x (sublist lo' hi' l) -> In x (sublist lo hi l).
+Proof.
+  intros.
+  apply sublist_In with (lo0 := lo' - lo)(hi0 := hi' - lo); rewrite sublist_sublist;
+    try split; try lia.
+  - repeat rewrite Z.sub_simpl_r; auto.
+  - destruct (Z_le_dec hi' lo'); try lia.
+    rewrite sublist_nil1 in *; auto; simpl in *; contradiction.
+Qed.
+
 Lemma mean_le : forall i j : Z,
  i <= j ->
  i <= i + ((j - i) / 2) <= j.
@@ -75,7 +214,69 @@ split.
   lia.
 Qed.
 
-Lemma body_search: semax_body Vprog Gprog f_binary_search binary_search_spec.
+Lemma Znth_lt_sublist_lt :
+  forall l i x key,
+    0 <= i < Zlength l ->
+    sorted l ->
+    Znth i l < key ->
+    In x (sublist 0 (i + 1) l) ->
+    x < key.
+Proof.
+intros.
+apply (In_sorted_range _ _ _ _ H0) in H2; try lia.
+assert (Hi: i + 1 - 1 = i) by lia.
+rewrite Hi in H2; clear Hi.
+lia.
+Qed.
+
+Lemma Znth_gt_sublist_gt :
+  forall l i x key,
+  0 <= i < Zlength l ->
+  sorted l ->
+  key < Znth i l ->
+  In x (sublist i (Zlength l) l) ->
+  key < x.
+Proof.
+intros.
+apply (In_sorted_range _ _ _ _ H0) in H2; try lia.
+Qed.
+
+Lemma sublist_lt_0 : forall low high (l : list Z),
+  low < 0 ->
+  sublist low high l = sublist 0 high l.
+Proof.
+intros.
+unfold sublist.
+rewrite Z2Nat_neg; auto.
+Qed.
+
+Lemma Forall_sublist_overlap : forall (l : list Z) P low high,  
+  high <= low ->
+  Forall P (sublist high (Zlength l) l) ->
+  Forall P (sublist low (Zlength l) l).
+Proof.
+intros l P low high Hle Hhigh.
+case (Z_lt_dec high 0); intros.
+  rewrite sublist_lt_0 in Hhigh; auto.
+  case (Z_lt_dec low 0); intros; [rewrite sublist_lt_0; auto|].  
+  apply Forall_forall.
+  intros.
+  assert (0 <= low) by lia.
+  pose proof (Forall_forall P (sublist 0 (Zlength l) l)) as [Hp1 Hp2].
+  specialize (Hp1 Hhigh).
+  apply Hp1.
+  revert H.
+  apply sublist_In_sublist; auto with zarith.
+assert (0 <= high) by lia.
+apply Forall_forall; intros.
+pose proof (Forall_forall P (sublist high (Zlength l) l)) as [Hp1 Hp2].
+specialize (Hp1 Hhigh).
+apply Hp1.
+revert H0.
+apply sublist_In_sublist; auto with zarith.
+Qed.
+  
+Lemma body_binary_search: semax_body Vprog Gprog f_binary_search binary_search_spec.
 Proof.
 start_function.
 forward.
@@ -96,42 +297,30 @@ forward_while (binary_search_while_spec a sh contents len key).
   * entailer!.
     split.
     + assert (Hle: low <= high) by lia.
-      pose proof (mean_le _ _  Hle) as Hdle.
+      pose proof (mean_le _ _  Hle) as Hdle.      
       assert (Heq: (high - low) / 2 = Int.signed (Int.divs (Int.repr (high - low)) (Int.repr 2))).
-        unfold Int.divs.
-        rewrite !Int.signed_repr.
-        -- rewrite Zquot.Zquot_Zdiv_pos by lia; reflexivity.
-        -- set (j := Int.min_signed) in *; compute in j; subst j.
-           set (j := Int.max_signed) in *; compute in j; subst j.
-           lia.
-        -- set (j := Int.min_signed) in *; compute in j; subst j.
-           set (j := Int.max_signed) in *; compute in j; subst j.
-           lia.
-        -- rewrite !Int.signed_repr;
-             set (j := Int.min_signed) in *; compute in j; subst j;
-             set (j := Int.max_signed) in *; compute in j; subst j; try lia.
-           rewrite Zquot.Zquot_Zdiv_pos by lia.
-           lia.
-        -- rewrite <- Heq.
-           set (j := Int.min_signed) in *; compute in j; subst j.
-           set (j := Int.max_signed) in *; compute in j; subst j.
-           lia.
+        unfold Int.divs; rewrite !Int.signed_repr; try rep_lia; [rewrite Zquot.Zquot_Zdiv_pos by lia; reflexivity|].
+        rewrite !Int.signed_repr; try rep_lia.
+        rewrite Zquot.Zquot_Zdiv_pos by lia.
+        rep_lia.
+      rewrite <- Heq.
+      rep_lia.
     + intro.
       destruct H0.
       unfold Int.mone in H11.
-      apply repr_inj_signed in H11; [congruence|idtac|idtac].
-      -- unfold repable_signed.
-         pose proof Int.min_signed_neg as Hneg.
-         set (j := Int.max_signed) in *; compute in j; subst j.
-         lia.
-      -- unfold repable_signed.
-         set (j := Int.min_signed) in *; compute in j; subst j.
-         set (j := Int.max_signed) in *; compute in j; subst j.
-         lia.
+      apply repr_inj_signed in H11; [congruence|unfold repable_signed|unfold repable_signed]; rep_lia.
    * assert_PROP (0 <= Int.unsigned (Int.add (Int.repr low) (Int.divs (Int.repr (high - low)) (Int.repr 2))) < Zlength (map Int.repr contents)).
        entailer!.
-       autorewrite with sublist.
-       admit.
+       autorewrite with sublist.       
+       assert (Hle: low <= high) by lia.
+       pose proof (mean_le _ _  Hle) as Hdle.
+       assert (Heq: low + (high - low) / 2 = Int.unsigned (Int.add (Int.repr low) (Int.divs (Int.repr (high - low)) (Int.repr 2)))).
+         unfold Int.divs; rewrite !Int.signed_repr; try rep_lia.
+         rewrite Zquot.Zquot_Zdiv_pos by lia.
+         rewrite add_repr.
+         rewrite !Int.unsigned_repr; auto.
+         rep_lia.
+       rewrite <- Heq; lia.
      assert_PROP ((0 <= Int.unsigned (Int.add (Int.repr low) (Int.divs (Int.repr (high - low)) (Int.repr 2))) < Zlength contents)).
        entailer!.
        autorewrite with sublist in *.
@@ -143,82 +332,132 @@ forward_while (binary_search_while_spec a sh contents len key).
            assert (Hle: low <= high) by lia.
            pose proof (mean_le _ _  Hle) as Hdle.
            assert (Heq: low + (high - low) / 2 = Int.signed (Int.add (Int.repr low) (Int.divs (Int.repr (high - low)) (Int.repr 2)))).
-             unfold Int.divs.
+             unfold Int.divs; rewrite !Int.signed_repr; try rep_lia.
              rewrite add_repr.
-             rewrite !Int.signed_repr.
-             ++ rewrite Zquot.Zquot_Zdiv_pos by lia; reflexivity.
-             ++ set (j := Int.min_signed) in *; compute in j; subst j.
-               set (j := Int.max_signed) in *; compute in j; subst j.
-               lia.
-             ++ set (j := Int.min_signed) in *; compute in j; subst j.
-               set (j := Int.max_signed) in *; compute in j; subst j.
-               lia.
-             ++ rewrite !Int.signed_repr;
-               set (j := Int.min_signed) in *; compute in j; subst j;
-               set (j := Int.max_signed) in *; compute in j; subst j; try lia.
-               rewrite Zquot.Zquot_Zdiv_pos by lia.
-               lia.
-             ++ rewrite <- Heq.
-               set (j := Int.min_signed) in *; compute in j; subst j.
-               set (j := Int.max_signed) in *; compute in j; subst j.
-               lia.
+             rewrite !Int.signed_repr; [rewrite Zquot.Zquot_Zdiv_pos by lia; reflexivity|].
+             rewrite Zquot.Zquot_Zdiv_pos by lia.
+             rep_lia.
+           rewrite <- Heq; rep_lia.
         ** entailer!.
            Exists ((low + ((high - low)/2)) + 1,high).
            entailer!.
            assert (Hle: low <= high) by lia.
            pose proof (mean_le _ _  Hle) as Hdle.
-           split; [lia|].           
-           admit.
+           split; [lia|].
+           assert (Heq: low + (high - low)/2 = Int.unsigned (Int.add (Int.repr low) (Int.divs (Int.repr (high - low)) (Int.repr 2)))).
+             unfold Int.divs; rewrite !Int.signed_repr; try rep_lia.
+             rewrite add_repr.
+             rewrite !Int.unsigned_repr; [rewrite Zquot.Zquot_Zdiv_pos by lia; reflexivity|].
+             rewrite Zquot.Zquot_Zdiv_pos by lia.
+             rep_lia.
+           rewrite <- Heq in H9,H10.
+           rewrite !Int.signed_repr in H10; [split; [|split]; intros|].
+           --- specialize (H6 H0).
+               eapply In_sorted_gt; eauto; lia.
+           --- specialize (H7 H0).
+               destruct H7 as [Hlow Hhigh].
+               split; [|assumption].
+               apply Forall_forall; intros.
+               eapply Znth_lt_sublist_lt; eauto.
+           --- f_equal.
+               unfold Int.add at 1.
+               f_equal.
+               rewrite <- Heq.
+               rewrite !Int.unsigned_repr; rep_lia.
+           --- assert (Hin: In (Znth (low + (high - low) / 2) contents) contents) by (eapply Znth_In; eauto).
+               pose proof (Forall_forall (fun x : Z => Int.min_signed <= x <= Int.max_signed) contents) as HFA.
+               simpl in HFA.
+               destruct HFA as [HFA1 HFA2].
+               apply (HFA1 H2 _ Hin).
       -- forward_if.
          ** forward.
             ++ entailer!.
               assert (Hle: low <= high) by lia.
               pose proof (mean_le _ _  Hle) as Hdle.
               assert (Heq: low + (high - low) / 2 = Int.signed (Int.add (Int.repr low) (Int.divs (Int.repr (high - low)) (Int.repr 2)))).
-                unfold Int.divs.
+                unfold Int.divs; rewrite !Int.signed_repr; try rep_lia.
                 rewrite add_repr.
-                rewrite !Int.signed_repr.
-                --- rewrite Zquot.Zquot_Zdiv_pos by lia; reflexivity.
-                --- set (j := Int.min_signed) in *; compute in j; subst j.
-                    set (j := Int.max_signed) in *; compute in j; subst j.
-                    lia.
-                --- set (j := Int.min_signed) in *; compute in j; subst j.
-                    set (j := Int.max_signed) in *; compute in j; subst j.
-                    lia.
-                --- rewrite !Int.signed_repr;
-                    set (j := Int.min_signed) in *; compute in j; subst j;
-                    set (j := Int.max_signed) in *; compute in j; subst j; try lia.
-                    rewrite Zquot.Zquot_Zdiv_pos by lia.
-                    lia.
-                --- rewrite <- Heq.
-                    set (j := Int.min_signed) in *; compute in j; subst j.
-                    set (j := Int.max_signed) in *; compute in j; subst j.
-                    lia.
+                rewrite !Int.signed_repr; [rewrite Zquot.Zquot_Zdiv_pos by lia; reflexivity|].
+                rewrite Zquot.Zquot_Zdiv_pos by lia.
+                rep_lia.
+              rewrite <- Heq; rep_lia.
             ++ entailer!.
               Exists (low,(low + ((high - low)/2)) - 1).
               entailer!.
               autorewrite with sublist in *.
               assert (Hle: low <= high) by lia.
               pose proof (mean_le _ _  Hle) as Hdle.
-              set (j := Int.min_signed) in *; compute in j; subst j.
-              split; [lia|].              
-              admit.
+              assert (Heq: low + (high - low)/2 = Int.unsigned (Int.add (Int.repr low) (Int.divs (Int.repr (high - low)) (Int.repr 2)))).
+                unfold Int.divs; rewrite !Int.signed_repr; try rep_lia.
+                rewrite add_repr.
+                rewrite !Int.unsigned_repr; [rewrite Zquot.Zquot_Zdiv_pos by lia; reflexivity|].
+                rewrite Zquot.Zquot_Zdiv_pos by lia.
+                rep_lia.
+              assert (Hle': Int.min_signed <= Znth (Int.unsigned (Int.add (Int.repr low) (Int.divs (Int.repr (high - low)) (Int.repr 2)))) contents <= Int.max_signed).
+                rewrite <- Heq.
+                assert (Hin: In (Znth (low + (high - low) / 2) contents) contents) by (eapply Znth_In; eauto; rewrite Heq; reflexivity).
+                pose proof (Forall_forall (fun x : Z => Int.min_signed <= x <= Int.max_signed) contents) as HFA.
+                simpl in HFA.
+                destruct HFA as [HFA1 HFA2].
+                apply (HFA1 H2 _ Hin).
+              rewrite !Int.signed_repr in H11; auto.
+              rewrite <- Heq in H11.
+              split; [rep_lia|]; split; [|split]; intros.
+              --- specialize (H6 H0).
+                  eapply (In_sorted_lt _ _ _ _ _ (high + 1)); eauto; lia.
+              --- specialize (H7 H0).
+                  destruct H7 as [Hl Hh].
+                  split; [assumption|].
+                  apply Forall_forall; intros.
+                  revert H7.
+                  apply Znth_gt_sublist_gt; auto.
+                  lia.
+              --- f_equal.
+                  unfold Int.sub.
+                  f_equal.
+                  rewrite !Int.unsigned_repr; [|rep_lia].
+                  rewrite <- Heq; reflexivity.
          ** forward.
             assert (H_key_eq:
              Int.signed (Int.repr (Znth (Int.unsigned (Int.add (Int.repr low) (Int.divs (Int.repr (high - low)) (Int.repr 2)))) contents)) = key) by lia.
             Exists (low + ((high - low) / 2)).
             entailer!.
+            assert (Hle: low <= high) by lia.
+            pose proof (mean_le _ _  Hle) as Hdle.
+            assert (Heq: low + (high - low) / 2 = Int.unsigned (Int.add (Int.repr low) (Int.divs (Int.repr (high - low)) (Int.repr 2)))).
+              unfold Int.divs; rewrite !Int.signed_repr; try rep_lia.
+              rewrite add_repr.
+              rewrite !Int.unsigned_repr; [rewrite Zquot.Zquot_Zdiv_pos by lia; reflexivity|].
+              rewrite Zquot.Zquot_Zdiv_pos by lia.
+              rep_lia.
+            assert (Hrange: Int.min_signed <= Znth (Int.unsigned (Int.add (Int.repr low) (Int.divs (Int.repr (high - low)) (Int.repr 2)))) contents <= Int.max_signed).
+              rewrite <- Heq.
+              assert (Hin: In (Znth (low + (high - low) / 2) contents) contents) by (eapply Znth_In; eauto; rewrite Heq; reflexivity).
+              pose proof (Forall_forall (fun x : Z => Int.min_signed <= x <= Int.max_signed) contents) as HFA.
+              simpl in HFA.
+              destruct HFA as [HFA1 HFA2].
+              apply (HFA1 H2 _ Hin).
             case (in_dec _ _); intro.
-            ++ autorewrite with sublist in *.
-              admit.
+            ++ split.
+              --- rewrite !Int.signed_repr; auto.
+                  rewrite <- Heq.
+                  reflexivity.
+              --- f_equal.                  
+                  rewrite Heq.
+                  unfold Int.add.
+                  f_equal.
+                  rewrite !Int.unsigned_repr; [reflexivity|idtac|rep_lia].
+                  unfold Int.divs; rewrite !Int.signed_repr; try rep_lia.
+                  rewrite !Int.unsigned_repr; rewrite Zquot.Zquot_Zdiv_pos; rep_lia.              
             ++ contradict n.
-              admit.
+              assert (Hin: In (Znth (low + (high - low) / 2) contents) contents) by (eapply Znth_In; eauto; rewrite Heq; reflexivity).
+              rewrite <- Heq.
+              rewrite !Int.signed_repr; auto.
+              rewrite Heq; auto.
 - forward.
   + entailer!.
-    set (j := Int.min_signed) in *; compute in j; subst j.
-    set (j := Int.max_signed) in *; compute in j; subst j.
     set (j := Int.signed Int.zero) in *; compute in j; subst j.
-    lia.
+    rep_lia.
   + Exists (-low - 1).
     entailer!.
     case (in_dec _ _); intro.
@@ -233,65 +472,29 @@ forward_while (binary_search_while_spec a sh contents len key).
       destruct H7.
       split; [lia|].
       split; auto.
-      admit.      
-Admitted.
-
-(*
-Lemma sorted_array_index_elt_le : 
-  (forall (intP_a_1_4_alloc_table_at_L:(alloc_table intP)),
-   (forall (intP_intM_a_1_4_at_L:(memory intP int32)),
-    (forall (a_1_0:(pointer intP)),
-     (forall (len_0_0:Z),
-      ((offset_min intP_a_1_4_alloc_table_at_L a_1_0) <= 0 /\
-       (offset_max intP_a_1_4_alloc_table_at_L a_1_0) >= (len_0_0 - 1) ->
-       ((sorted a_1_0 0 (len_0_0 - 1) intP_intM_a_1_4_at_L) ->
-        (forall (i_3:Z),
-         (forall (j_0:Z),
-          (0 <= i_3 /\ i_3 <= (len_0_0 - 1) ->
-           (0 <= j_0 /\ j_0 <= (len_0_0 - 1) ->
-            (i_3 <= j_0 ->
-             (integer_of_int32
-              (select intP_intM_a_1_4_at_L (shift a_1_0 i_3))) <=
-             (integer_of_int32
-              (select intP_intM_a_1_4_at_L (shift a_1_0 j_0)))))))))))))).
-Proof.
-move => alloc_table mem a len [H_min H_max] H_srt i j.
-move: i.
-elim/(well_founded_ind (Zwf_well_founded 0)): j.
-move => x H_ind i H_x H_j H_ix.
-have H_ltx: i = x \/ i < x by omega.
-elim H_ltx => H_ltx'; first by rewrite H_ltx'; auto with zarith.  
-suff H_lt: integer_of_int32 (select mem (shift a (x-1))) <= integer_of_int32 (select mem (shift a x)).
-- suff H_ltm: integer_of_int32 (select mem (shift a i)) <= integer_of_int32 (select mem (shift a (x-1))) by auto with zarith.
-  by apply H_ind; rewrite /Zwf; auto with zarith.
-- pose proof (H_srt (x-1)) as H_ran.
-  move: H_ran.
-  have ->: x - 1 + 1 = x by auto with zarith.
-  move => H_ran.
-  by apply H_ran; auto with zarith.
+      assert (Hle: high + 1 <= low) by lia.
+      eapply Forall_sublist_overlap; eauto.
 Qed.
 
-Lemma sorted_array_index_lt : 
-  (forall (intP_a_2_5_alloc_table_at_L:(alloc_table intP)),
-   (forall (intP_intM_a_2_5_at_L:(memory intP int32)),
-    (forall (a_2:(pointer intP)),
-     (forall (len_1:Z),
-      ((offset_min intP_a_2_5_alloc_table_at_L a_2) <= 0 /\
-       (offset_max intP_a_2_5_alloc_table_at_L a_2) >= (len_1 - 1) ->
-       ((sorted a_2 0 (len_1 - 1) intP_intM_a_2_5_at_L) ->
-        (forall (i_4:Z),
-         (forall (j_1:Z),
-          (0 <= i_4 /\ i_4 <= (len_1 - 1) ->
-           (0 <= j_1 /\ j_1 <= (len_1 - 1) ->
-            ((integer_of_int32 (select intP_intM_a_2_5_at_L (shift a_2 i_4))) <
-             (integer_of_int32 (select intP_intM_a_2_5_at_L (shift a_2 j_1))) ->
-             i_4 < j_1))))))))))).
+Definition four_contents := [1; 2; 3; 4].
+
+Lemma body_main : semax_body Vprog Gprog f_main main_spec.
 Proof.
-move => alloc_table mem a len H_ran H_srt i j H_lei H_lej.
-elim (Z_lt_ge_dec i j) => H_dec; first by [].
-have H_ji: j <= i by auto with zarith.
-have H_le_le: integer_of_int32 (select mem (shift a j)) <= integer_of_int32 (select mem (shift a i)).
-  by apply (sorted_array_index_elt_le _ _ _ _ H_ran H_srt _ _ H_lej H_lei).
-by move => H_lt; auto with zarith.
+  start_function.
+  forward_call (gv _four,Ews,four_contents,4,3).
+  { split. auto.
+    change (Zlength four_contents) with 4.
+    repeat constructor; computable.
+  }
+  Intro r; forward.
 Qed.
-*)
+
+Existing Instance NullExtension.Espec.
+
+Lemma prog_correct:
+  semax_prog prog tt Vprog Gprog.
+Proof.
+prove_semax_prog.
+semax_func_cons body_binary_search.
+semax_func_cons body_main.
+Qed.
